{
 "cells": [
  {
   "cell_type": "markdown",
   "metadata": {},
   "source": [
    "---\n",
    "\n",
    "## Exercises for Students\n",
    "\n",
    "$$\n",
    "\\left\\{\\begin{array}{c}{x+2 y-2 z=4} \\\\ {2 x+y+z=0} \\\\ {3 x+2 y+z=1}\\end{array}\\right.\\quad\n",
    "\\left\\{\\begin{array}{c}{x+y+z-t=2} \\\\ {2 x+y+z=3} \\\\ {-x+z-t=0} \\\\ {3 x+2 y-z+2 t=-1}\\end{array}\\right.\\quad\n",
    "\\left\\{\\begin{array}{c}{x+y-z-t=0} \\\\ {2 x+3 y-2 z+t=4} \\\\ {3 x+5 z=0} \\\\ {-x+y-3 z+2 t=3}\\end{array}\\right.\n",
    "$$"
   ]
  },
  {
   "cell_type": "markdown",
   "metadata": {},
   "source": [
    "$$\n",
    "\\text{1. For the system of equations:}\n",
    "\\left\\{\n",
    "\\begin{array}{l}\n",
    "x + 2y - 2z = 4 \\\\\n",
    "2x + y + z = 0 \\\\\n",
    "3x + 2y + z = 1\n",
    "\\end{array}\n",
    "\\right.\n",
    "$$\n",
    "\n",
    "First, subtract the second equation from the third equation to eliminate \\( y \\):\n",
    "$$\n",
    "(3x + 2y + z) - (2x + y + z) = 1 - 0\n",
    "$$\n",
    "Simplifying:\n",
    "$$\n",
    "x + y = 1 \\quad \\Rightarrow \\quad y = 1 - x\n",
    "$$\n",
    "\n",
    "Substitute \\( y = 1 - x \\) into the second equation:\n",
    "$$\n",
    "2x + (1 - x) + z = 0\n",
    "$$\n",
    "Simplifying:\n",
    "$$\n",
    "x + z = -1 \\quad \\Rightarrow \\quad z = -1 - x\n",
    "$$\n",
    "\n",
    "Now substitute \\( y = 1 - x \\) and \\( z = -1 - x \\) into the first equation:\n",
    "$$\n",
    "x + 2(1 - x) - 2(-1 - x) = 4\n",
    "$$\n",
    "Simplifying:\n",
    "$$\n",
    "x + 2 - 2x + 2 + 2x = 4 \\quad \\Rightarrow \\quad x + 4 = 4 \\quad \\Rightarrow \\quad x = 0\n",
    "$$\n",
    "\n",
    "Substitute \\( x = 0 \\) into \\( y = 1 - x \\) and \\( z = -1 - x \\):\n",
    "$$\n",
    "y = 1, \\quad z = -1\n",
    "$$\n",
    "\n",
    "Thus, the solution is:\n",
    "$$\n",
    "x = 0, \\quad y = 1, \\quad z = -1\n",
    "$$\n",
    "\n",
    "$$\n",
    "\\text{2. For the second system of equations:}\n",
    "\\left\\{\n",
    "\\begin{array}{l}\n",
    "x + y + z - t = 2 \\\\\n",
    "2x + y + z = 3 \\\\\n",
    "-x + z - t = 0 \\\\\n",
    "3x + 2y - z + 2t = -1\n",
    "\\end{array}\n",
    "\\right.\n",
    "$$\n",
    "\n",
    "First, subtract the second equation from the first:\n",
    "$$\n",
    "(x + y + z - t) - (2x + y + z) = 2 - 3\n",
    "$$\n",
    "Simplifying:\n",
    "$$\n",
    "-x - t = -1 \\quad \\Rightarrow \\quad x + t = 1 \\quad \\Rightarrow \\quad t = 1 - x\n",
    "$$\n",
    "\n",
    "Next, substitute \\( t = 1 - x \\) into the third equation:\n",
    "$$\n",
    "-x + z - (1 - x) = 0\n",
    "$$\n",
    "Simplifying:\n",
    "$$\n",
    "-x + z - 1 + x = 0 \\quad \\Rightarrow \\quad z = 1\n",
    "$$\n",
    "\n",
    "Substitute \\( z = 1 \\) and \\( t = 1 - x \\) into the second equation:\n",
    "$$\n",
    "2x + y + 1 = 3 \\quad \\Rightarrow \\quad 2x + y = 2 \\quad \\Rightarrow \\quad y = 2 - 2x\n",
    "$$\n",
    "\n",
    "Substitute \\( z = 1 \\), \\( t = 1 - x \\), and \\( y = 2 - 2x \\) into the fourth equation:\n",
    "$$\n",
    "3x + 2(2 - 2x) - 1 + 2(1 - x) = -1\n",
    "$$\n",
    "Simplifying:\n",
    "$$\n",
    "3x + 4 - 4x - 1 + 2 - 2x = -1 \\quad \\Rightarrow \\quad -3x + 5 = -1 \\quad \\Rightarrow \\quad -3x = -6 \\quad \\Rightarrow \\quad x = 2\n",
    "$$\n",
    "\n",
    "Substitute \\( x = 2 \\) into \\( y = 2 - 2x \\), \\( z = 1 \\), and \\( t = 1 - x \\):\n",
    "$$\n",
    "y = -2, \\quad z = 1, \\quad t = -1\n",
    "$$\n",
    "\n",
    "Thus, the solution is:\n",
    "$$\n",
    "x = 2, \\quad y = -2, \\quad z = 1, \\quad t = -1\n",
    "$$\n",
    "\n",
    "$$\n",
    "\\text{3. For the third system of equations:}\n",
    "\\left\\{\n",
    "\\begin{array}{l}\n",
    "x + y - z - t = 0 \\\\\n",
    "2x + 3y - 2z + t = 4 \\\\\n",
    "3x + 5z = 0 \\\\\n",
    "-x + y - 3z + 2t = 3\n",
    "\\end{array}\n",
    "\\right.\n",
    "$$\n",
    "\n",
    "From the third equation, solve for \\( x \\):\n",
    "$$\n",
    "3x + 5z = 0 \\quad \\Rightarrow \\quad x = -\\frac{5}{3}z\n",
    "$$\n",
    "\n",
    "Substitute \\( x = -\\frac{5}{3}z \\) into the first equation:\n",
    "$$\n",
    "-\\frac{5}{3}z + y - z - t = 0\n",
    "$$\n",
    "Simplifying:\n",
    "$$\n",
    "y - \\frac{8}{3}z - t = 0 \\quad \\Rightarrow \\quad y = \\frac{8}{3}z + t\n",
    "$$\n",
    "\n",
    "Substitute \\( x = -\\frac{5}{3}z \\) and \\( y = \\frac{8}{3}z + t \\) into the second equation:\n",
    "$$\n",
    "2\\left(-\\frac{5}{3}z\\right) + 3\\left(\\frac{8}{3}z + t\\right) - 2z + t = 4\n",
    "$$\n",
    "Simplifying:\n",
    "$$\n",
    "-\\frac{10}{3}z + 8z + 3t - 2z + t = 4\n",
    "$$\n",
    "Combining terms:\n",
    "$$\n",
    "\\frac{14}{3}z + 4t = 4 \\quad \\Rightarrow \\quad 14z + 12t = 12\n",
    "$$\n",
    "Simplifying:\n",
    "$$\n",
    "7z + 6t = 6\n",
    "$$\n",
    "\n",
    "Now substitute \\( x = -\\frac{5}{3}z \\) and \\( y = \\frac{8}{3}z + t \\) into the fourth equation:\n",
    "$$\n",
    "-\\left(-\\frac{5}{3}z\\right) + \\left(\\frac{8}{3}z + t\\right) - 3z + 2t = 3\n",
    "$$\n",
    "Simplifying:\n",
    "$$\n",
    "\\frac{5}{3}z + \\frac{8}{3}z + t - 3z + 2t = 3 \\quad \\Rightarrow \\quad \\frac{13}{3}z + 3t = 3\n",
    "$$\n",
    "Multiplying through by 3:\n",
    "$$\n",
    "13z + 9t = 9\n",
    "$$\n",
    "\n",
    "Solve the system:\n",
    "$$\n",
    "7z + 6t = 6 \\quad \\text{(1)}\n",
    "$$\n",
    "$$\n",
    "13z + 9t = 9 \\quad \\text{(2)}\n",
    "$$\n",
    "\n",
    "Multiply equation (1) by 3:\n",
    "$$\n",
    "21z + 18t = 18 \\quad \\text{(3)}\n",
    "$$\n",
    "Multiply equation (2) by 2:\n",
    "$$\n",
    "26z + 18t = 18 \\quad \\text{(4)}\n",
    "$$\n",
    "Subtract equation (3) from equation (4):\n",
    "$$\n",
    "5z = 0 \\quad \\Rightarrow \\quad z = 0\n",
    "$$\n",
    "\n",
    "Substitute \\( z = 0 \\) into equations (1) and (2):\n",
    "$$\n",
    "7(0) + 6t = 6 \\quad \\Rightarrow \\quad 6t = 6 \\quad \\Rightarrow \\quad t = 1\n",
    "$$\n",
    "\n",
    "Substitute \\( z = 0 \\) and \\( t = 1 \\) into the expressions for \\( x \\) and \\( y \\):\n",
    "$$\n",
    "x = -\\frac{5}{3}(0) = 0, \\quad y = \\frac{8}{3}(0) + 1 = 1\n",
    "$$\n",
    "\n",
    "Thus, the solution is:\n",
    "$$\n",
    "x = 0, \\quad y = 1, \\quad z = 0, \\quad t = 1\n",
    "$$\n"
   ]
  }
 ],
 "metadata": {
  "language_info": {
   "name": "python"
  }
 },
 "nbformat": 4,
 "nbformat_minor": 2
}
